\documentclass[11pt]{article}

\usepackage{amssymb}
\usepackage{wasysym}
\usepackage{tipa}


\begin{document}

\title{Exercise 7}
\author{Jeremy Nguyen}
\date{\today}
\maketitle

$a \gtrsim b \lesssim c$

$\aleph \beth \gimel \otimes$

\mercury, \earth

$\female \male \taurus \boxminus$
\textschwa

$\frac{a}{b}$

$\frac{\frac{a}{b}}{\frac{c+d}{d+e}}$

$F = G_{N}\frac{m_{1}m_{2}}{r^2}$

$n\pm(E,T)=\frac{1}{e^{\frac{E}{k_{B}T}}\pm1}=\frac{1}{e^{{\hbar\omega/k_{B}T}}\pm1}$

$F\mu = [D_{\mu}, D_{v}] =
	\partial_{\mu}A_{v} - \partial_{V}A_{\mu} =
	\partial_{[\mu}A_{v]} $

% \[\frac12a+b\]
% \[\tfrac12a+b\]

\[\frac{df}{dt}\]
\[\frac{\partial f}{\partial t}\]
\[\int f(x) dx, \sum x_n, \prod \omega_k\int_0^1 f(x)dx, \sum_{n=0}^7
	x_n, \prod_1^{10} \omega_k\]
$\int_0^1 f(x)dx, \sum_{n=0}^7 x_n, \prod_1^{10} \omega_k$

\center
Taylor expansion $e^x = \sum_\infty^b \frac{1}{n!}x^{n}$.

\[\int_{0}^{1} \frac{df}{dx} = f(1) - f(0)\]
\[e^{\zeta(s)} = \prod_{n=1}^\infty e^(1/n^s)\]

\end{document}